ITPDemo.lean
@@ -6,13 +6,12 @@ import AutomaticProofGeneralization.Formalizations.irrationality_of_sqrts
 import AutomaticProofGeneralization.Formalizations.impossible_graphs
 
 open Autogeneralize
-
 open Real
 open Lean Elab Tactic Meta Term Command
 
-set_option linter.unusedVariables false
 set_option pp.showLetValues false
 set_option autoImplicit false
+-- set_option trace.ProofPrinting true
 
 /- - - - - - - - - - - - - - - - - - - - - - - - - - - - - - - - - - - -
 Generalization of the proof that √17 is irrational
@@ -41,12 +40,12 @@ example: ∀ (p n : ℕ), Nat.Prime p → Irrational (√p + n) := by
   intros p n p_prime
 
   /- Start with the theorem that √17 is irrational. -/
-  let irrat_sqrt : Irrational (sqrt (17:ℕ)+17) := by {apply Irrational.add_nat; apply irrat_def; intros h; obtain ⟨a, b, ⟨copr, h⟩⟩ := h; have a_div : 17 ∣ a := by {have c := (Nat.Prime.dvd_mul (prime_seventeen)).mp ((by apply (Iff.mpr dvd_iff_exists_eq_mul_right); use (b*b); rw [← mul_assoc]; rw [h];): 17 ∣ a*a); cases c; assumption; assumption}; have a_is_pk : ∃ k, a = 17 * k := by {apply (Iff.mp dvd_iff_exists_eq_mul_right) a_div}; obtain ⟨k, hk⟩ := a_is_pk; rw [hk] at h; replace h := Eq.symm h; rw [mul_assoc] at h; rw [mul_assoc] at h; rw [mul_comm 17 k] at h; rw [mul_eq_mul_left_iff] at h; rw [← mul_assoc k k 17] at h; have := Nat.Prime.ne_zero prime_seventeen; cases h with | inl => have b_div : 17 ∣ b := by {have c := (Nat.Prime.dvd_mul (prime_seventeen)).mp ((by apply (Iff.mpr dvd_iff_exists_eq_mul_left); use (k*k))); cases c; assumption; assumption}; have p_dvd_gcd : 17 ∣ Nat.gcd a b := by {apply Iff.mpr Nat.dvd_gcd_iff ⟨a_div, b_div⟩}; clear a_div b_div; rw [copr] at p_dvd_gcd; apply Nat.Prime.not_dvd_one (prime_seventeen) p_dvd_gcd | inr => apply this; assumption}
+  let irrat_sum_sqrt : Irrational (sqrt (17:ℕ)+17) := by {apply Irrational.add_nat; apply irrat_def; intros h; obtain ⟨a, b, ⟨copr, h⟩⟩ := h; have a_div : 17 ∣ a := by {have c := (Nat.Prime.dvd_mul (prime_seventeen)).mp ((by apply (Iff.mpr dvd_iff_exists_eq_mul_right); use (b*b); rw [← mul_assoc]; rw [h];): 17 ∣ a*a); cases c; assumption; assumption}; have a_is_pk : ∃ k, a = 17 * k := by {apply (Iff.mp dvd_iff_exists_eq_mul_right) a_div}; obtain ⟨k, hk⟩ := a_is_pk; rw [hk] at h; replace h := Eq.symm h; rw [mul_assoc] at h; rw [mul_assoc] at h; rw [mul_comm 17 k] at h; rw [mul_eq_mul_left_iff] at h; rw [← mul_assoc k k 17] at h; have := Nat.Prime.ne_zero prime_seventeen; cases h with | inl => have b_div : 17 ∣ b := by {have c := (Nat.Prime.dvd_mul (prime_seventeen)).mp ((by apply (Iff.mpr dvd_iff_exists_eq_mul_left); use (k*k))); cases c; assumption; assumption}; have p_dvd_gcd : 17 ∣ Nat.gcd a b := by {apply Iff.mpr Nat.dvd_gcd_iff ⟨a_div, b_div⟩}; clear a_div b_div; rw [copr] at p_dvd_gcd; apply Nat.Prime.not_dvd_one (prime_seventeen) p_dvd_gcd | inr => apply this; assumption}
 
   /- Find the proof-based generalization, and add it as a theorem in the context. -/
-  autogeneralize (17:ℕ) in irrat_sqrt
+  autogeneralize (17:ℕ) in irrat_sum_sqrt
 
-  exact irrat_sqrt.Gen p p_prime n
+  exact irrat_sum_sqrt.Gen p p_prime n
 
 /- - - - - - - - - - - - - - - - - - - - - - - - - - - - - - - - - - - -
 A demonstration of robust generalization of _dependent_ uses of a constant.
@@ -56,11 +55,11 @@ Generalization of the proof that |A ∪ B| ≤ 4 when |A|=2 and |B|=2
 to the proof that |A ∪ B| ≤ n+m when |A|=n and |B|=m
 - - - - - - - - - - - - - - - - - - - - - - - - - - - - - - - - - - - - -/
 
-example : ∀ (n m : ℕ) (α : Type) [inst : Fintype α] [inst_2 : DecidableEq α] (A B : Finset α),
+example : ∀ (n m : ℕ) (α : Type) [Fintype α] [DecidableEq α] (A B : Finset α),
   A.card = n → B.card = m → (A ∪ B).card ≤ n+m:= by
 
   /- Start with the theorem that |A ∪ B| ≤ 4 when |A|=2 and |B|=2. -/
-  let union_of_finsets (α : Type) [inst : Fintype α] [inst_2 : DecidableEq α] (A B : Finset α) (hA : A.card = 2) (hB : B.card = 2) : (A ∪ B).card ≤ 4 := by apply hA ▸ hB ▸ Finset.card_union_add_card_inter A B ▸ Nat.le_add_right _ _
+  let union_of_finsets (α : Type) [Fintype α] [DecidableEq α] (A B : Finset α) (hA : A.card = 2) (hB : B.card = 2) : (A ∪ B).card ≤ 4 := by apply hA ▸ hB ▸ Finset.card_union_add_card_inter A B ▸ Nat.le_add_right _ _
 
   /- Find the proof-based generalization, and add it as a theorem in the context. -/
   autogeneralize (2:ℕ) in union_of_finsets
@@ -76,7 +75,7 @@ to the proof that no n-vertex graph has degree sequence (1, n-1, n-1, ..., n-1) 
 (Note that when n=2, a graph with degree sequence (1,1) exists)
 - - - - - - - - - - - - - - - - - - - - - - - - - - - - - - - - - - - - -/
 example :
-  ∀ (n : ℕ), 2 < n → ∀ (G : SimpleGraph (Fin n)) [inst : DecidableRel G.Adj],
+  ∀ (n : ℕ), 2 < n → ∀ (G : SimpleGraph (Fin n)) [DecidableRel G.Adj],
   (∃ v, G.degree v = 1 ∧ ∀ (w : Fin n), w ≠ v → G.degree w = n - 1) → False
 := by
   intro n hn
